Refactor TensorExprSyntax and move semantics into TensorExprSemantics

theories/TensorAutomation/Aux_stdpp.v
@@ -72,3 +72,860 @@ Proof.
       destruct a as [a|]; [|easy].
       exists (a :: l'); cbn; congruence.
 Qed.
+
+
+From stdpp Require Import strings fin_maps pmap gmap hlist.
+From stdpp Require Import pretty.
+
+(* FIXME: Move to Aux_stdpp *)
+Lemma bind_is_Some {A B} (f : A -> option B) (mx : option A) : 
+  is_Some (mx ≫= f) <-> is_Some mx /\ forall x, mx = Some x -> is_Some (f x).
+Proof.
+  destruct mx.
+  - cbn.
+    naive_solver.
+  - cbn.
+    rewrite 2 is_Some_alt.
+    firstorder.
+Qed.
+
+Ltac f_equal_let :=
+  let H := fresh in 
+  match goal with 
+  | |- (let '_ := ?x in _) = (let '_ := ?y in _) => 
+    enough (H : x = y) by now first [rewrite H | rewrite <- H]
+  | |- (let _ := ?x in _) = (let _ := ?y in _) => 
+    enough (H : x = y) by now first [rewrite H | rewrite <- H]
+  end.
+
+
+Lemma lookup_insert_case `{FinMap K M} {A} (m : M A) (i j : K) (x : A) : 
+  <[i:=x]> m !! j = if decide (i = j) then Some x else m !! j.
+Proof.
+  case_decide; now simplify_map_eq.
+Qed.
+
+Lemma NoDup_fmap_iff {A B} (f : A -> B) (l : list A) : 
+  NoDup (f <$> l) <->
+  NoDup l /\
+  forall a a', a ∈ l -> a' ∈ l -> f a = f a' -> a = a'.
+Proof.
+  split; [|intros []; now apply NoDup_fmap_2_strong].
+  intros Hmap.
+  split; [now apply NoDup_fmap_1 in Hmap|].
+  intros a a' (ia & Hia)%elem_of_list_lookup (ia' & Hia')%elem_of_list_lookup.
+  intros Hfas.
+  enough (ia = ia') by congruence.
+  apply (NoDup_lookup (f <$> l) _ _ (f a) Hmap);
+  rewrite list_lookup_fmap;
+  [now rewrite Hia|].
+  now rewrite Hia', Hfas.
+Qed.
+
+Lemma fsts_prod_map {A B C D} (f : A -> C) (g : B -> D) (l : list (A * B)) : 
+  (prod_map f g <$> l).*1 = f <$> (l.*1).
+Proof.
+  rewrite <- 2 list_fmap_compose.
+  reflexivity.
+Qed.
+
+Lemma snds_prod_map {A B C D} (f : A -> C) (g : B -> D) (l : list (A * B)) : 
+  (prod_map f g <$> l).*2 = g <$> (l.*2).
+Proof.
+  rewrite <- 2 list_fmap_compose.
+  reflexivity.
+Qed.
+
+  
+
+Lemma disjoint_difference_l
+  `{Set_ A C} `{!RelDecision (@elem_of A C _)} (X Y Z : C) : 
+  X ∖ Y ## Z <-> X ∩ Z ⊆ Y. 
+Proof.
+  split; [set_solver|].
+  intros HXZ x.
+  set_solver.
+Qed.
+
+Lemma disjoint_difference_symm
+  `{Set_ A C} (X Y Z : C) : 
+  X ∖ Y ## Z <-> X ## Z ∖ Y.
+Proof.
+  set_solver.
+Qed.
+
+
+Lemma not_elem_of_drop_iff {A} (l : list A) a i :
+  a ∉ drop i l <->
+  (forall j a', i <= j -> l !! j = Some a' -> a' <> a).
+Proof.
+  rewrite elem_of_list_lookup.
+  setoid_rewrite lookup_drop.
+  split.
+  - intros Hnex j a' Hij Hlook ->.
+    apply Hnex.
+    exists (j - i).
+    rewrite <- Hlook.
+    f_equal; lia.
+  - intros Hlook (j & Hj).
+    apply (Hlook (i + j) a); [lia|easy|easy].
+Qed.
+
+Lemma not_elem_of_drop_S_iff {A} (l : list A) a i :
+  a ∉ drop (S i) l <->
+  (forall j a', i < j -> l !! j = Some a' -> a' <> a).
+Proof.
+  apply not_elem_of_drop_iff.
+Qed.
+
+
+Lemma list_nil_iff {A} (l : list A) : l = [] <-> l ≡ [].
+Proof.
+  split; [now intros ->|].
+  intros Hl.
+  destruct l; set_solver.
+Qed.
+
+Lemma NoDup_list_eq_singleton_iff {A} (l : list A) a : NoDup l ->
+  l = [a] <-> l ≡ [a].
+Proof.
+  intros Hdup.
+  split; [intros ->; set_solver|].
+  intros Hl.
+  destruct l as [|a' l]; [set_solver|].
+  rewrite NoDup_cons in Hdup.
+  f_equal; [set_solver|].
+  apply list_nil_iff.
+  intros x.
+  split; [|easy].
+  intros Hx.
+  assert (x ∈ [a]) as ->%elem_of_list_singleton by now rewrite <- Hl; right.
+  enough (a' = a) by now subst.
+  apply elem_of_list_singleton.
+  now rewrite <- Hl; left.
+Qed.
+
+Lemma NoDup_list_eq_singleton_iff' {A} (l : list A) a : NoDup l ->
+  l = [a] <-> a ∈ l /\ (forall b, b ∈ l -> b = a).
+Proof.
+  intros Hdup.
+  rewrite NoDup_list_eq_singleton_iff by easy.
+  set_solver.
+Qed.
+
+Lemma last_filter_Some `{P : A -> Prop} `{∀ a, Decision (P a)} l a :
+  last (filter P l) = Some a <-> exists i, l !! i = Some a /\ P a /\ forall j a', i < j -> 
+    l !! j = Some a' -> ~ P a'.
+Proof.
+  split.
+  1: {
+    revert a;
+    induction l as [|a' l IHl]; [easy|]; intros a.
+    cbn.
+    case_decide as HPa'.
+    - rewrite last_cons.
+      destruct (last (filter P l)) as [a''|] eqn:Hlf.
+      + intros [= ->].
+        specialize (IHl a eq_refl) as (i & Hi & HPa & Higt).
+        exists (S i).
+        split; [apply Hi|].
+        split; [easy|].
+        intros [|j] ab Hij; [lia|].
+        apply Higt; lia.
+      + intros [= ->].
+        exists 0.
+        split; [easy|].
+        split; [easy|].
+        intros [|j] a' Hj; [lia|].
+        cbn.
+        intros Hlj HPa.
+        rewrite last_None in Hlf.
+        apply (elem_of_nil a').
+        rewrite <- Hlf.
+        apply elem_of_list_filter.
+        split; [easy|].
+        now apply elem_of_list_lookup_2 in Hlj.
+    - intros (i & Hi & HPa & Hgt)%IHl.
+      exists (S i).
+      split; [easy|].
+      split; [easy|].
+      intros [|j] a'' Hj; [lia|].
+      cbn.
+      apply Hgt; lia.
+  }
+  1:{
+    intros (i & Hi & HPa & Hnotin).
+    revert l Hi Hnotin;
+    induction i; intros l Hi Hnotin.
+    - destruct l; [easy|].
+      cbn in Hi.
+      injection Hi; intros ->.
+      cbn.
+      rewrite decide_True by easy.
+      rewrite last_cons.
+      rewrite (fun H => proj2 (last_None _) H); [easy|].
+      apply list_nil_iff.
+      intros x.
+      rewrite elem_of_nil.
+      split; [|easy].
+      rewrite elem_of_list_filter.
+      rewrite elem_of_list_lookup.
+      intros (Px & j & Hj).
+      specialize (Hnotin (S j) x ltac:(lia) Hj).
+      easy.
+    - destruct l as [|a' l]; [easy|].
+      cbn.
+      cbn in Hi.
+      case_decide; [|apply IHi; [easy|]; intros j ? ?; apply (Hnotin (S j)); lia].
+      rewrite last_cons.
+      destruct (last (filter P l)) as [lst|] eqn:Hlst.
+      + rewrite <- Hlst.
+        apply IHi; [easy|].
+        intros j ? ?; apply (Hnotin (S j)); lia.
+      + exfalso.
+        apply last_None in Hlst.
+        apply (filter_nil_not_elem_of _ _ _ Hlst HPa).
+        now apply elem_of_list_lookup_2 in Hi.
+  }
+Qed.
+
+
+Definition finv {A B C} `{Elements A C}
+  `{EqDecision B} `{Inhabited A}
+  (dom : C) (f : A -> B) : B -> A :=
+  fun b => 
+    default inhabitant (
+      head (filter (fun a => f a = b) (elements dom))
+    ).
+
+Lemma finv_right_inverse {A B C} `{FinSet A C} `{Inhabited A} `{EqDecision B}
+  (dom : C) (f : A -> B) b : (exists a, a ∈ dom /\ f a = b) ->
+    f (finv dom f b) = b.
+Proof.
+  intros (a & Hadom & Hfa).
+  unfold finv.
+  destruct (head (filter (λ a, f a = b) (elements dom))) as [a'|] eqn:Hfilt.
+  - apply head_Some_elem_of, elem_of_list_filter in Hfilt.
+    easy.
+  - exfalso.
+    apply head_None in Hfilt.
+    rewrite <- (elem_of_nil a), <- Hfilt.
+    apply elem_of_list_filter; set_solver.
+Qed.
+
+Lemma finv_double_left_inverse {A B C} `{FinSet A C} `{Inhabited A} `{EqDecision B}
+  (dom : C) (f : A -> B) a : a ∈ dom ->
+    f (finv dom f (f a)) = f a.
+Proof.
+  intros Hadom.
+  apply finv_right_inverse; eauto.
+Qed.
+
+Lemma finv_left_inverse {A B C} `{FinSet A C} `{Inhabited A} `{EqDecision B}
+  (dom : C) (f : A -> B) a : a ∈ dom -> 
+    (forall a a', a ∈ dom -> a' ∈ dom -> f a = f a' -> a = a') ->
+    finv dom f (f a) = a.
+Proof.
+  intros Hadom Hfinj.
+  unfold finv.
+  replace (filter (λ a', f a' = f a) (elements dom)) with [a]; [easy|].
+  symmetry.
+  apply NoDup_list_eq_singleton_iff'; [apply NoDup_filter, NoDup_elements|].
+  split; [now apply elem_of_list_filter; split; [|apply elem_of_elements]|].
+  intros b (Hfb & Hbdom%elem_of_elements)%elem_of_list_filter.
+  auto.
+Qed.
+
+
+
+Lemma app_inj_len_l {A} (l m l' m' : list A) : 
+  length l = length l' -> 
+  l ++ m = l' ++ m' -> 
+  l = l' /\ m = m'.
+Proof.
+  intros Hlen Heq.
+  apply (f_equal (take (length l))) in Heq as Heql.
+  rewrite take_app_length, Hlen, take_app_length in Heql.
+  subst l'.
+  split; [easy|].
+  now apply app_inv_head in Heq.
+Qed.
+
+Lemma app_inj_len_r {A} (l m l' m' : list A) : 
+  length m = length m' -> 
+  l ++ m = l' ++ m' -> 
+  l = l' /\ m = m'.
+Proof.
+  intros Hlen Heq.
+  specialize (f_equal length Heq).
+  simpl_list.
+  intros Hlens.
+  apply app_inj_len_l; easy + lia.
+Qed.
+
+
+
+Lemma list_to_set_concat {A C} `{Set_ A C} (l : list (list A)) : 
+  list_to_set (concat l) ≡@{C} ⋃ (list_to_set <$> l).
+Proof.
+  induction l; [reflexivity|].
+  now cbn; rewrite list_to_set_app, IHl.
+Qed.
+
+Lemma list_to_set_concat_L {A C} `{Set_ A C} `{!LeibnizEquiv C} (l : list (list A)) : 
+  list_to_set (concat l) =@{C} ⋃ (list_to_set <$> l).
+Proof.
+  unfold_leibniz.
+  apply list_to_set_concat.
+Qed.
+
+
+
+Lemma NoDup_list_bind {A B} (f : A -> list B) l : 
+  NoDup l -> 
+    (forall a, a ∈ l -> NoDup (f a)) ->
+    (forall a a' b, a ∈ l -> a' ∈ l -> a <> a' -> 
+      b ∈ f a -> b ∉ f a') ->
+  NoDup (l ≫= f).
+Proof.
+  intros Hdup Hfdup Hinj.
+  induction Hdup; [constructor|].
+  cbn.
+  apply NoDup_app.
+  split; [now apply Hfdup; left|].
+  split; [|apply IHHdup; set_solver].
+  intros b Hbx.
+  rewrite elem_of_list_bind.
+  intros (y & Hby & Hy).
+  revert Hbx Hby.
+  apply Hinj; set_solver.
+Qed.
+
+
+
+Lemma map_img_list_to_map `{FinMap K M} `{Set_ A SA} 
+  (l : list (K * A)) : 
+  NoDup l.*1 ->
+  map_img (list_to_map l :> M A) ≡@{SA} list_to_set l.*2.
+Proof.
+  intros Hl.
+  rewrite map_img_alt.
+  now rewrite map_to_list_to_map by easy.
+Qed.
+
+Lemma map_img_list_to_map_L `{FinMap K M} `{Set_ A SA} `{!LeibnizEquiv SA}
+  (l : list (K * A)) : 
+  NoDup l.*1 ->
+  map_img (list_to_map l :> M A) =@{SA} list_to_set l.*2.
+Proof.
+  unfold_leibniz.
+  apply map_img_list_to_map.
+Qed.
+
+
+
+
+Fixpoint list_decomps_aux {A} (pre l : list A) : list (list A * A * list A) :=
+  match l with 
+  | [] => []
+  | a :: l => 
+    (pre, a, l) :: list_decomps_aux (pre ++ [a]) l
+  end.
+
+Definition list_decomps {A} (l : list A) : list (list A * A * list A) :=
+  list_decomps_aux [] l.
+  
+
+Lemma elem_of_list_decomps_aux {A} (pre l : list A) : 
+  forall hd a tl, (hd, a, tl) ∈ list_decomps_aux pre l <->
+    hd ++ [a] ++ tl = pre ++ l /\
+    length (pre) <= length (hd).
+Proof.
+  revert pre; induction l; intros pre hd b tl.
+  - cbn.
+    split; [easy|].
+    intros (Heq%(f_equal length) & Hlen).
+    revert Heq.
+    simpl_list.
+    cbn.
+    lia.
+  - cbn.
+    rewrite elem_of_cons.
+    rewrite IHl.
+    split.
+    + intros [[= -> -> ->] | [Heq Hlen]]; [easy|].
+      rewrite <- app_assoc in Heq.
+      split; [apply Heq|].
+      rewrite <- Hlen.
+      simpl_list; cbn; lia.
+    + intros [Heq Hlen].
+      destruct_decide (decide (length pre = length hd)) as Hleneq.
+      * left.
+        apply app_inj_len_l in Heq; [|easy].
+        now destruct Heq as [-> [= -> ->]].
+      * right.
+        rewrite <- app_assoc.
+        split; [easy|].
+        simpl_list; cbn; lia.
+Qed.
+
+Lemma elem_of_list_decomps {A} (l : list A) : 
+  forall hd a tl, (hd, a, tl) ∈ list_decomps l <->
+    hd ++ [a] ++ tl = l.
+Proof.
+  intros hd a tl.
+  unfold list_decomps.
+  rewrite elem_of_list_decomps_aux.
+  naive_solver lia.
+Qed.
+
+(* FIXME: Move *)
+Lemma exists_pair {A B} (P : A * B -> Prop) : 
+  (exists ab, P ab) <-> exists a, exists b, P (a, b).
+Proof.
+  split.
+  - intros [[] ?]; eauto.
+  - intros (?&?&?); eauto.
+Qed.
+
+Definition list_removals {A} (l : list A) : list (A * list A) :=
+  (λ '(hd, a, tl), (a, hd ++ tl)) <$> list_decomps l.
+
+Lemma elem_of_list_removals {A} (l : list A) a hd_tl : 
+  (a, hd_tl) ∈ list_removals l <-> exists hd tl, hd_tl = hd ++ tl /\ 
+    hd ++ [a] ++ tl = l.
+Proof.
+  unfold list_removals.
+  rewrite elem_of_list_fmap.
+  rewrite 2 exists_pair.
+  setoid_rewrite pair_eq.
+  setoid_rewrite elem_of_list_decomps.
+  naive_solver.
+Qed.
+
+
+Lemma elem_of_list_removals_perm {A} (l : list A) a hd_tl : 
+  (a, hd_tl) ∈ list_removals l -> l ≡ₚ a :: hd_tl.
+Proof.
+  rewrite elem_of_list_removals.
+  intros (hd & tl & -> & <-).
+  quote_Permutation.
+  apply rlist.eval_Permutation.
+  cbn.
+  compute_done.
+Qed.
+
+Definition list_select `(P : A -> Prop)
+  `{forall (a : A), Decision (P a)} (l : list A) : list (A * list A) :=
+  filter (fun a_rst => P (fst a_rst)) (list_removals l).
+
+
+Lemma elem_of_list_select {A} `(P : A -> Prop)
+  `{forall (a : A), Decision (P a)} (l : list A) a hd_tl : 
+  (a, hd_tl) ∈ list_select P l <-> P a /\ exists hd tl, hd_tl = hd ++ tl /\ 
+    hd ++ [a] ++ tl = l.
+Proof.
+  unfold list_select.
+  rewrite elem_of_list_filter.
+  now rewrite elem_of_list_removals.
+Qed.
+
+
+Lemma elem_of_list_select_perm {A} `(P : A -> Prop)
+  `{forall (a : A), Decision (P a)} (l : list A) a hd_tl : 
+  (a, hd_tl) ∈ list_select P l -> l ≡ₚ a :: hd_tl.
+Proof. 
+  intros [_ (? & ? & -> & <-)]%elem_of_list_select.
+  solve_Permutation.
+Qed. 
+
+
+Definition gmap_map `{Countable A} (m : gmap A A) : A -> A :=
+  fun a => default a (m !! a).
+
+Lemma gmap_map_correct `{Countable A} (m : gmap A A) a b : 
+  m !! a = Some b -> gmap_map m a = b.
+Proof.
+  unfold gmap_map.
+  now intros ->.
+Qed.
+
+Lemma gmap_map_idemp `{Countable A} (m : gmap A A) a : 
+  a ∉ dom m -> gmap_map m a = a.
+Proof.
+  intros Ha.
+  unfold gmap_map.
+  unfold default.
+  case_match eqn:Heq; [|reflexivity].
+  now apply elem_of_dom_2 in Heq.
+Qed.
+
+
+
+Lemma elem_of_from_option_list_singleton {A} (a : A) (ma : option A) : 
+  a ∈ from_option (λ x, [x]) [] ma <->
+  ma = Some a.
+Proof.
+  destruct ma; cbn; set_solver.
+Qed.
+
+
+Lemma filter_with_iff_neg_Permutation {A} {P Q : A -> Prop} 
+  `{∀ a, Decision (P a)} `{∀ a, Decision (Q a)} l : 
+  (∀ a, P a <-> ~ Q a) -> 
+  filter P l ++ filter Q l ≡ₚ l.
+Proof.
+  intros HPQ.
+  induction l; [easy|].
+  cbn.
+  case_decide.
+  - rewrite decide_False by now apply HPQ.
+    cbn.
+    now rewrite IHl.
+  - case_decide; [|exfalso; naive_solver].
+    rewrite <- IHl at 3.
+    solve_Permutation.
+Qed.
+
+Lemma filter_with_neg_Permutation {A} {P : A -> Prop} 
+  `{∀ a, Decision (P a)} l : 
+  filter P l ++ filter (λ a, ~ P a) l ≡ₚ l.
+Proof.
+  rewrite Permutation_app_comm.
+  now apply filter_with_iff_neg_Permutation.
+Qed.
+
+Lemma filter_neg_with_Permutation {A} {P : A -> Prop} 
+  `{∀ a, Decision (P a)} l : 
+  filter (λ a, ~ P a) l ++ filter P l ≡ₚ l.
+Proof.
+  now apply filter_with_iff_neg_Permutation.
+Qed.
+
+
+
+Lemma fmap_Permuation_iff_exists {A B} (f : A -> B) (l : list A) l' : 
+  f <$> l ≡ₚ l' <-> 
+  exists l'', l ≡ₚ l'' /\ f <$> l'' = l'.
+Proof.
+  split.
+  - revert l'; induction l as [|a l IHl]; intros l'.
+    + cbn.
+      intros ->%Permutation_nil.
+      eauto.
+    + cbn.
+      intros Hperm.
+      assert (Hal' : f a ∈ l') by now rewrite <- Hperm; left.
+      apply elem_of_list_split in Hal' as Ha'l'.
+      destruct Ha'l' as (fl'1 & fl'2 & Heq).
+      subst l'.
+      specialize (IHl (fl'1 ++ fl'2) (Permutation_cons_app_inv _ _ Hperm)).
+      destruct IHl as (l'' & Hl & Hfl'').
+      apply fmap_app_inv in Hfl'' as (l'1 & l'2 & Hl'1 & Hl'2 & Hl'').
+      exists (l'1 ++ a :: l'2).
+      split; [rewrite Hl; subst; solve_Permutation|].
+      rewrite fmap_app; cbn.
+      congruence.
+  - intros (? & Hperm & Heq).
+    now rewrite Hperm, <- Heq.
+Qed.
+
+
+Lemma size_map_img_le_size_dom `{FinMapDom K M SK}
+  `{!Elements K SK} `{!FinSet K SK} `{FinSet A SA} (m : M A) : 
+  size (map_img m :> SA) <= size (dom m).
+Proof.
+  induction m using map_first_key_ind.
+  - now rewrite map_img_empty, dom_empty, 2 size_empty.
+  - rewrite dom_insert.
+    assert (Hid : i ∉ dom m) by (now apply not_elem_of_dom).
+    rewrite size_union by set_solver.
+    rewrite size_singleton.
+    transitivity (1 + size (map_img m :> SA))%nat; [|lia].
+    etransitivity; [eapply subseteq_size; apply map_img_insert_subseteq|].
+    rewrite size_union_alt, size_singleton.
+    apply Nat.add_le_mono_l.
+    apply subseteq_size, subseteq_difference_l; reflexivity.
+Qed.
+
+Lemma map_dom_img_lt_card_iff `{FinMapDom K M SK}
+  `{!Elements K SK} `{!FinSet K SK} `{FinSet A SA} `{!RelDecision (∈@{SA})}
+    (m : M A) : 
+  size (map_img m :> SA) < size (dom m) <-> 
+  exists i j a, m !! i = Some a /\ m !! j = Some a /\ i <> j.
+Proof.
+  split.
+  - induction m using map_first_key_ind; 
+    [now rewrite dom_empty, map_img_empty, 2 size_empty|].
+    rewrite dom_insert, map_img_insert_notin by easy.
+    assert (Hid : i ∉ dom m) by (now apply not_elem_of_dom).
+    destruct_decide (decide (x ∈@{SA} map_img m)) as Hx.
+    + apply elem_of_map_img_1 in Hx as (j & Hj).
+      intros _.
+      exists i, j, x.
+      enough (i <> j) by now 
+      rewrite lookup_insert, lookup_insert_ne.
+      intros ->.
+      now apply elem_of_dom_2 in Hj.
+    + rewrite 2 (size_union {[_]}) by set_solver.
+      rewrite 2 size_singleton.
+      intros (j & k & a & Hj & Hk & Hjk)%Nat.succ_lt_mono%IHm.
+      exists j, k, a.
+      rewrite lookup_insert_ne by (intros ->; now apply elem_of_dom_2 in Hj).
+      rewrite lookup_insert_ne by (intros ->; now apply elem_of_dom_2 in Hk).
+      easy.
+  - intros (i & j & a & Hi & Hj & Hij).
+    rewrite <- (insert_delete m i a Hi).
+    rewrite map_img_insert_notin, dom_insert by apply lookup_delete.
+    rewrite <- (insert_delete (delete i m) j a) by now rewrite lookup_delete_ne.
+    rewrite map_img_insert_notin, dom_insert by apply lookup_delete.
+    rewrite (union_assoc _), (union_idemp _).
+    rewrite size_union_alt, 
+      (size_union {[i]}), (size_union {[j]}), 3 size_singleton by set_solver.
+    eapply Nat.le_lt_trans; [apply -> Nat.succ_le_mono; 
+      apply subseteq_size, subseteq_difference_l; reflexivity|].
+    pose proof (size_map_img_le_size_dom (delete j (delete i m)) (SA:=SA)).
+    lia.
+Qed.
+
+Lemma map_dom_img_eq_card_iff_inj `{FinMapDom K M SK}
+  `{!Elements K SK} `{!FinSet K SK} `{FinSet A SA} `{!RelDecision (∈@{SA})}
+    (m : M A) : 
+  size (dom m) = size (map_img m :> SA) <-> 
+  forall i j a, m !! i = Some a -> m !! j = Some a -> i = j.
+Proof.
+  split.
+  - intros Hsize.
+    assert (Hn : ~ size (map_img m :> SA) < size (dom m)) by lia.
+    rewrite map_dom_img_lt_card_iff in Hn.
+    intros i j a Hi Hj.
+    apply dec_stable.
+    intros Hij.
+    apply Hn.
+    naive_solver.
+  - intros Hinj.
+    specialize (size_map_img_le_size_dom m (SA:=SA)).
+    enough (~ size (map_img m :> SA) < size (dom m)) by lia.
+    rewrite map_dom_img_lt_card_iff.
+    naive_solver.
+Qed.
+
+Lemma map_dom_img_eq_card_iff_NoDup `{FinMapDom K M SK}
+  `{!Elements K SK} `{!FinSet K SK} `{FinSet A SA} `{!RelDecision (∈@{SA})}
+    (m : M A) : 
+  size (dom m) = size (map_img m :> SA) <-> 
+  NoDup (map_to_list m).*2.
+Proof.
+  rewrite map_dom_img_eq_card_iff_inj.
+  rewrite NoDup_alt.
+  setoid_rewrite list_lookup_fmap.
+  setoid_rewrite fmap_Some.
+  split.
+  - intros Hinj i j a.
+    intros ([k a'] & Hk & Ha') ([k' a''] & Hk' & Ha'').
+    cbn in Ha', Ha''.
+    subst a' a''.
+    apply elem_of_list_lookup_2 in Hk as Hka.
+    apply elem_of_list_lookup_2 in Hk' as Hk'a.
+    rewrite elem_of_map_to_list in * |-.
+    assert (k = k') by eauto.
+    subst k'.
+    now apply (NoDup_lookup _ _ _ (k,a) (NoDup_map_to_list m)).
+  - intros HNoDup.
+    intros k k' a Hka Hk'a.
+    apply elem_of_map_to_list in Hka as Hka'.
+    apply elem_of_map_to_list in Hk'a as Hk'a'.
+    apply elem_of_list_lookup_1 in Hka' as [i Hi].
+    apply elem_of_list_lookup_1 in Hk'a' as [j Hj].
+    enough (i = j) by congruence.
+    apply (HNoDup _ _ a); eexists (_, a); eauto.
+Qed.
+
+
+Lemma elem_of_list_fmap_prod_map {A B C D} 
+  (f : A -> C) (g : B -> D) (l : list (A * B)) cd : 
+  cd ∈ prod_map f g <$> l <-> 
+  exists a b, (a, b) ∈ l /\ f a = cd.1 /\ g b = cd.2.
+Proof.
+  destruct cd as [c d].
+  rewrite elem_of_list_fmap.
+  rewrite exists_pair.
+  cbn.
+  naive_solver.
+Qed.
+
+Lemma fsts_prod_swap {A B} (l : list (A * B)) : 
+  (prod_swap <$> l).*1 = l.*2.
+Proof.
+  induction l as [|[]]; cbn; f_equal; easy.
+Qed.
+
+Lemma snds_prod_swap {A B} (l : list (A * B)) : 
+  (prod_swap <$> l).*2 = l.*1.
+Proof.
+  induction l as [|[]]; cbn; f_equal; easy.
+Qed.
+
+Lemma lookup_list_to_map_gen `{FinMap K M} {A} 
+  (l : list (K * A)) k : 
+    (list_to_map l :> M A) !! k = snd <$> head (filter (λ kv, kv.1 = k) l).
+Proof.
+  induction l as [|[k' a'] l IHl].
+  - cbn.
+    now rewrite lookup_empty.
+  - cbn.
+    rewrite lookup_insert_case.
+    case_decide; [reflexivity|].
+    apply IHl.
+Qed.
+
+Lemma list_to_map_eq_fold_right `{FinMap K M} {A} 
+  (l : list (K * A)) : (list_to_map l :> M A) = foldr (λ p, <[p.1:=p.2]>) ∅ l.
+Proof.
+  induction l; cbn; f_equal; congruence.
+Qed.
+
+
+Lemma gmap_map_inj_on `{Countable A} (m : gmap A A) (X : gset A) : 
+  (forall i j a, m !! i = Some a -> m !! j = Some a -> i = j) -> 
+  X ⊆ dom m -> 
+  forall a b, a ∈ X -> b ∈ X -> gmap_map m a = gmap_map m b -> a = b.
+Proof.
+  intros Hinj HX a b [ma Hma]%HX%elem_of_dom [mb Hmb]%HX%elem_of_dom.
+  rewrite (gmap_map_correct _ _ _ Hma), (gmap_map_correct _ _ _ Hmb).
+  intros ->.
+  eauto.
+Qed.
+
+
+Lemma list_to_set_equiv `{SemiSet A C} (l l' : list A) : 
+  list_to_set l ≡@{C} list_to_set l' <-> l ≡ l'.
+Proof.
+  rewrite set_equiv.
+  setoid_rewrite elem_of_list_to_set.
+  reflexivity.
+Qed.
+
+Lemma list_to_set_subseteq `{SemiSet A C} (l l' : list A) : 
+  list_to_set l ⊆@{C} list_to_set l' <-> l ⊆ l'.
+Proof.
+  unfold subseteq, set_subseteq_instance, list_subseteq.
+  setoid_rewrite elem_of_list_to_set.
+  reflexivity.
+Qed.
+
+
+Notation "'unfold' x" := (ltac:(let x' := eval unfold x in x in 
+  exact (eq_refl : x = x'))) (at level 10, only parsing).
+
+
+Lemma decide_not `{HNP : Decision (~ P)} `{HP : Decision P} {A} (x y : A) : 
+  (if @decide (~ P) HNP then x else y) = 
+  (if @decide P HP then y else x).
+Proof.
+  now do 2 case_decide.
+Qed.
+
+
+
+Notation gset_to_Pset s := 
+  (list_to_set (C:=Pset) $ strings.string_to_pos <$> elements s).
+
+
+Lemma elem_of_gset_string_to_Pset (s : gset string) p : 
+  p ∈@{Pset} gset_to_Pset s <->
+  exists y, y ∈ s /\ p = encode y.
+Proof.
+  rewrite elem_of_list_to_set, elem_of_list_fmap.
+  setoid_rewrite elem_of_elements.
+  naive_solver.
+Qed.
+
+Lemma elem_of_gset_string_to_Pset' (s : gset string) (x : string) :
+  encode x ∈ gset_to_Pset s <-> x ∈ s.
+Proof.
+  rewrite elem_of_gset_string_to_Pset.
+  naive_solver.
+Qed.
+
+Lemma gset_to_Pset_inj (s s' : gset string) : 
+  gset_to_Pset s = gset_to_Pset s' -> s = s'.
+Proof.
+  intros Heq.
+  apply set_eq; intros x.
+  by rewrite <- 2 elem_of_gset_string_to_Pset', Heq.
+Qed.
+
+
+Lemma list_bind_ext_strong {A B} (f g : A -> list B) (l : list A) :
+  (forall a, a ∈ l -> f a = g a) ->
+  l ≫= f = l ≫= g.
+Proof.
+  induction l; [reflexivity|];
+  intros Hfg.
+  cbn.
+  rewrite Hfg by now left.
+  f_equal.
+  apply IHl; intros; apply Hfg; now right.
+Qed.
+
+Lemma caps_eq_r_weaken `{FinSet A SA} (X Y Z Z' : SA) : 
+  Z ⊆ Z' -> X ∩ Z' ≡ Y ∩ Z' -> X ∩ Z ≡ Y ∩ Z.
+Proof.
+  set_solver.
+Qed.
+
+Lemma caps_eq_r_weaken_L `{FinSet A SA} `{!LeibnizEquiv SA} (X Y Z Z' : SA) : 
+  Z ⊆ Z' -> X ∩ Z' = Y ∩ Z' -> X ∩ Z = Y ∩ Z.
+Proof.
+  unfold_leibniz.
+  apply caps_eq_r_weaken.
+Qed.
+
+
+Lemma guard_is_Some `{Decision P} {A} (x : A) : 
+  is_Some (guard P ≫= λ _, Some x) <-> P.
+Proof.
+  case_guard; cbn; [done|]; by split; [intros ?%is_Some_None|].
+Qed.
+
+Lemma list_fmap_filter_inv 
+  `(f : A -> B) (g : B -> A) `{!Cancel eq g f} 
+  {P : A -> Prop} `{∀ a, Decision (P a)} l : 
+  f <$> filter P l =@{list B} filter (P ∘ g) (f <$> l).
+Proof.
+  induction l; [done|].
+  cbn.
+  rewrite (decide_ext (P (g _)) (P a)) by 
+    now rewrite (cancel g f).
+  unfold filter in *.
+  rewrite <- IHl.
+  by case_decide.
+Qed.
+
+Lemma list_filter_fmap 
+  `(f : A -> B)
+  {P : B -> Prop} `{∀ a, Decision (P a)} l : 
+  filter P (f <$> l) =@{list B} f <$> filter (P ∘ f) l.
+Proof.
+  induction l; [done|].
+  cbn.
+  by case_decide;
+  unfold filter in *;
+  rewrite IHl.
+Qed.
+
+Lemma list_filter_iff_strong {A} (P1 P2 : A -> Prop)
+  `{∀ a, Decision (P1 a)} `{∀ a, Decision (P2 a)} (l : list A) : 
+  (∀ a, a ∈ l -> P1 a <-> P2 a) ->
+  filter P1 l = filter P2 l.
+Proof.
+  unfold filter.
+  induction l; [done|].
+  intros HP.
+  cbn.
+  unfold filter.
+  erewrite decide_ext by now apply HP; left.
+  rewrite IHl by now intros; apply HP; right.
+  reflexivity.
+Qed.
